demo/mutrec/MutrecAproof.v
@@ -1,0 +1,222 @@
+Require Import CoqlibC Maps Postorder.
+Require Import AST Linking.
+Require Import ValuesC Memory GlobalenvsC Events Smallstep.
+Require Import Op Registers ClightC Renumber.
+Require Import CtypesC CtypingC.
+Require Import sflib.
+Require Import IntegersC.
+
+Require Import MutrecHeader.
+Require Import MutrecA MutrecAspec.
+Require Import Simulation.
+Require Import Skeleton Mod ModSem SimMod SimModSem SimSymb SimMem AsmregsC MatchSimModSem.
+Require SimMemInjC.
+Require SoundTop.
+Require Import Clightdefs.
+
+Set Implicit Arguments.
+
+Section SIMMODSEM.
+
+Variable skenv_link: SkEnv.t.
+Variable sm_link: SimMem.t.
+Let md_src: Mod.t := (MutrecAspec.module prog).
+Let md_tgt: Mod.t := (ClightC.module2 prog).
+Hypothesis (INCLSRC: SkEnv.includes skenv_link md_src.(Mod.sk)).
+Hypothesis (INCLTGT: SkEnv.includes skenv_link md_tgt.(Mod.sk)).
+Hypothesis (WF: SkEnv.wf skenv_link).
+Let ge := Build_genv (SkEnv.revive (SkEnv.project skenv_link md_src.(Mod.sk)) prog) prog.(prog_comp_env).
+Let tge := Build_genv (SkEnv.revive (SkEnv.project skenv_link md_tgt.(Mod.sk)) prog) prog.(prog_comp_env).
+Definition msp: ModSemPair.t := ModSemPair.mk (md_src skenv_link) (md_tgt skenv_link) tt sm_link.
+
+Inductive match_states_internal: MutrecAspec.state -> Clight.state -> Prop :=
+| match_callstate_nonzero
+    i m_src m_tgt
+    fptr
+    (* targs tres cconv *)
+  :
+    match_states_internal (Callstate i m_src) (Clight.Callstate fptr (Tfunction (* targs tres cconv) *)
+                                                                        (Tcons tint Tnil) tint cc_default)
+                                                                [Vint i] Kstop m_tgt)
+| match_returnstate
+    i m_src m_tgt
+  :
+    match_states_internal (Returnstate i m_src) (Clight.Returnstate (Vint i) Kstop m_tgt)
+.
+
+Inductive match_states (sm_init: SimMem.t)
+          (idx: nat) (st_src0: MutrecAspec.state) (st_tgt0: Clight.state) (sm0: SimMem.t): Prop :=
+| match_states_intro
+    (MATCHST: match_states_internal st_src0 st_tgt0)
+    (MCOMPATSRC: st_src0.(get_mem) = sm0.(SimMem.src))
+    (MCOMPATTGT: st_tgt0.(ClightC.get_mem) = sm0.(SimMem.tgt))
+    (MWF: SimMemInj.wf' sm0)
+.
+
+Theorem make_match_genvs :
+  SimSymbId.sim_skenv (SkEnv.project skenv_link md_src.(Mod.sk)) (SkEnv.project skenv_link md_tgt.(Mod.sk)) ->
+  Genv.match_genvs (match_globdef (fun _ => eq) eq tt) ge tge.
+Proof.
+  subst_locals. ss. ii.
+  eapply SimSymbId.sim_skenv_revive; eauto.
+  admit "ez - reflexivity".
+Qed.
+
+Theorem sim_modsem
+  :
+    ModSemPair.sim msp
+.
+Proof.
+  eapply match_states_sim with (match_states := match_states) (match_states_at := top4) (sound_state := SoundTop.sound_state);
+    eauto; ii; ss.
+  - instantiate (1:= Nat.lt). apply lt_wf.
+  - eapply SoundTop.sound_state_local_preservation.
+  - (* init bsim *)
+    destruct sm_arg; ss. clarify.
+    inv SIMARGS; ss. clarify.
+    inv INITTGT.
+    hexploit (SimMemInjC.skenv_inject_revive prog); et. { apply SIMSKENV. } intro SIMSKENV0; des.
+    exploit make_match_genvs; eauto. { apply SIMSKENV. } intro SIMGE. des.
+    eexists. eexists (SimMemInj.mk _ _ _ _ _ _ _).
+    esplits; eauto.
+    + econs; eauto with mem; ss.
+      eapply SimMemInj.frozen_refl.
+    + inv SAFESRC. destruct args_src, args_tgt; ss. clarify.
+      econs; ss; eauto.
+      inv VALS. inv H1. inv H3.
+      assert(fd = func_f).
+      {
+        clear - FINDF.
+        uge. des_ifs.
+        unfold SkEnv.revive, SkEnv.project in Heq. ss.
+        rewrite MapsC.PTree_filter_map_spec in *.
+        unfold o_bind, o_join, o_map in Heq. des_ifs.
+        clear - Heq2.
+        unfold prog in *. unfold Clightdefs.mkprogram in *. ss.
+        unfold prog_defmap in *. ss. unfold global_definitions in *.
+        apply PTree_Properties.in_of_list in Heq2.
+        ss. des; clarify.
+      } clarify.
+      assert(tvs = [Vint i]).
+      {
+        unfold signature_of_function in TYP. ss.
+        inv TYP. ss. cbn. unfold typify. des_ifs; ss.
+      } clarify.
+      econs; eauto.
+  - (* init progress *)
+    des. inv SAFESRC.
+    inv SIMARGS; ss.
+    hexploit (SimMemInjC.skenv_inject_revive prog); et. { apply SIMSKENV. } intro SIMSKENV0; des.
+    exploit make_match_genvs; eauto. { apply SIMSKENV. } intro SIMGE.
+
+    (* exploit (Genv.find_funct_match_genv SIMGE); eauto. i; des. ss. clarify. folder. *)
+    hexploit (@fsim_external_inject_eq); try apply FINDF; eauto. clear FPTR. intro FPTR.
+
+    (* exploit (Genv.find_funct_match_genv SIMGE); eauto. i; des. ss. clarify. folder. *)
+    (* inv TYP. *)
+    esplits; eauto. econs; eauto.
+    + rewrite <- FPTR. eauto.
+    + instantiate (1:= [Vint i]). rewrite VS in *. inv VALS. inv H3. inv H2. econs; ss.
+      cbn. unfold typify. des_ifs; ss.
+  - (* call wf *)
+    inv MATCH; ss.
+  - (* call fsim *)
+    (* hexploit (SimMemInjC.skenv_inject_revive prog); et. { apply SIMSKENV. } intro SIMSKENV0; des. *)
+    (* exploit make_match_genvs; eauto. { apply SIMSKENV. } intro SIMGE. des. *)
+    (* inv MATCH; ss. destruct sm0; ss. clarify. *)
+    (* inv CALLSRC. inv MATCHST; ss. *)
+    (* folder. *)
+    (* (* inv MCOMPAT; ss. clear_tac. *) *)
+    (* (* exploit (fsim_external_funct_inject SIMGE); eauto. { ii; clarify; ss. des; ss. } intro EXTTGT. *) *)
+    (* esplits; eauto. *)
+    (* + econs; eauto. *)
+    (*   * des. clarify. esplits; eauto. *)
+    (*     (* exploit (sim_internal_funct_inject SIMGE); try apply SIG; et. *) *)
+
+    (*     (* Arguments sim_internal_funct_inject [_]. *) *)
+    (*     (* destruct SIMSKENVLINK. inv H.  rr in SIMSKENV1. clarify. *) *)
+    (*     (* exploit (sim_internal_funct_inject); try apply VAL; try apply SIG; et. *) *)
+    (*     (* { erewrite match_globdef_eq. eapply Global_match_genvs_refl. } *) *)
+    (*     (* { inv SIMSKENV. ss. } *) *)
+
+    (*     (***************** TODO: Add as a lemma in GlobalenvsC. *******************) *)
+    (*     inv SIMSKENV. *)
+    (*     assert(fptr_arg = tv). *)
+    (*     { eapply fsim_external_inject_eq; try apply SIG; et. Undo 1. *)
+    (*       inv VAL; ss. des_ifs_safe. apply Genv.find_funct_ptr_iff in SIG. unfold Genv.find_def in *. *)
+    (*       inv SIMSKE. ss. inv INJECT; ss. *)
+    (*       exploit (DOMAIN b1); eauto. *)
+    (*       { eapply Genv.genv_defs_range; et. } *)
+    (*       i; clarify. *)
+    (*     } *)
+    (*     clarify. *)
+    (* + ss. *)
+    (* + reflexivity. *)
+    admit "".
+
+  - (* after fsim *)
+    hexploit (SimMemInjC.skenv_inject_revive prog); et. { apply SIMSKENV. } intro SIMSKENV0; des.
+    exploit make_match_genvs; eauto. { apply SIMSKENV. } intro SIMGE. des.
+    inv AFTERSRC.
+    inv SIMRET. ss. exists (SimMemInj.unlift' sm_arg sm_ret). destruct sm_ret; ss. clarify.
+    inv MATCH; ss. inv MATCHST; ss.
+    inv HISTORY. ss. clear_tac.
+    esplits; eauto.
+    + econs; eauto.
+    + econs; ss; eauto. destruct retv_src, retv_tgt; ss. clarify.
+      inv MLE0; ss.
+      (* inv MCOMPAT. clear_tac. *)
+      inv RETV. unfold typify. des_ifs; ss.
+      econs; eauto.
+    + refl.
+
+  - (* final fsim *)
+    inv MATCH. inv FINALSRC; inv MATCHST; ss.
+    (* inv MCONT_EXT. inv MCOMPAT; ss. *)
+    clarify.
+    eexists sm0. esplits; ss; eauto.
+    + econs; eauto. ss.
+    + refl.
+  - left; i.
+    exploit make_match_genvs; eauto. { apply SIMSKENV. } intro SIMGE. des.
+
+    esplits; eauto.
+    { apply modsem1_receptive. }
+    inv MATCH.
+    ii. hexploit (@step_simulation prog skenv_link skenv_link); eauto; ss.
+    i; des.
+    esplits; eauto.
+    + left. eapply spread_dplus; eauto. eapply modsem2_determinate; eauto.
+    + econs; ss.
+      * inv H0; ss; inv MCOMPAT; ss.
+      * inv H0; ss; inv MCOMPAT; ss.
+
+Unshelve.
+  all: ss; try (by econs).
+Qed.
+
+End SIMMODSEM.
+
+
+
+
+Section SIMMOD.
+
+Variables prog tprog: program.
+Hypothesis TRANSL: match_prog prog tprog.
+Definition mp: ModPair.t := ModPair.mk (RTLC.module prog) (RTLC.module tprog) tt.
+
+Theorem sim_mod
+  :
+    ModPair.sim mp
+.
+Proof.
+  econs; ss.
+  - r. eapply Sk.match_program_eq; eauto.
+    ii. destruct f1; ss.
+    + clarify. right. esplits; eauto.
+    + clarify. left. esplits; eauto.
+  - ii. inv SIMSKENVLINK. eapply sim_modsem; eauto.
+Qed.
+
+End SIMMOD.
